Seem to have got it working for liftdoors

inference-tool/src/main/scala/inference/Dirties.scala
@@ -479,7 +479,7 @@ object Dirties {
     //     }
     //   }
     // }
-    //
+
     // Log.root.debug("Seeds:")
     // for (seed <- seeds) {
     //   val fitness = deap_gp.fitness(seed, training_set, pset)
